Gt3/JEq/Wk.lean
@@ -40,9 +40,9 @@ theorem Ctx.JEq.psub {Γ Δ} (h : PSub Γ Δ) {A a b : Tm 0} (hab : JEq Δ A a b
       apply_assumption
       · exact hL
       · apply h.cons' hΓ
-        <;> first | assumption | apply JEq.lhs_is_ty
-        <;> (first | apply JEq.nats | apply_assumption) <;>
-        first | assumption | exact h.left_ok | exact h.right_ok
+        <;> (first | assumption | apply IsTy.not | apply JEq.lhs_is_ty)
+        <;> (first | apply JEq.nats | apply_assumption)
+        <;> first | assumption | exact h.left_ok | exact h.right_ok
     }
     | apply h.is_perm; assumption
 
