Gt3/Syntax/Logic.lean
@@ -1,0 +1,25 @@
+import Gt3.Syntax.Subst
+
+def Tm.imp {k} (φ ψ : Tm k) : Tm k := .trunc (.arr φ ψ)
+
+def Tm.and {k} (φ ψ : Tm k) : Tm k := .trunc (.prod φ ψ)
+
+def Tm.not {k} (φ : Tm k) : Tm k := .eqn φ .empty
+
+def Tm.or {k} (φ ψ : Tm k) : Tm k := .imp (.not φ) ψ
+
+@[simp]
+theorem Tm.open_imp {k} (φ ψ : Tm (k + 1)) (x : String)
+  : (φ.imp ψ).open x = (φ.open x).imp (ψ.open x) := by simp [imp]
+
+@[simp]
+theorem Tm.open_and {k} (φ ψ : Tm (k + 1)) (x : String)
+  : (φ.and ψ).open x = (φ.open x).and (ψ.open x) := by simp [and]
+
+@[simp]
+theorem Tm.open_not {k} (φ : Tm (k + 1)) (x : String)
+  : φ.not.open x = (φ.open x).not := by simp [not]
+
+@[simp]
+theorem Tm.open_or {k} (φ ψ : Tm (k + 1)) (x : String)
+  : (φ.or ψ).open x = (φ.open x).or (ψ.open x) := by simp [or]
